theories/Spilling/RLiveMin.v
@@ -1,0 +1,103 @@
+Require Import List Map Env AllInRel Exp MoreList.
+Require Import IL Annotation.
+Require Import Liveness.Liveness.
+Require Import ExpVarsBounded SpillSound SpillUtil.
+
+
+
+Set Implicit Arguments.
+
+
+
+Definition is_rlive_min k ZL Λ s sl Rlv
+  := forall R M, spill_sound k ZL Λ (R,M) s sl
+                 -> Rlv ⊆ R
+.
+
+
+Inductive rlive_min (k:nat)
+  : list params -> list (⦃var⦄ * ⦃var⦄) -> ⦃var⦄ -> stmt -> spilling -> ann ⦃var⦄ -> Prop :=
+| RMinLet ZL Λ x e s an sl Rlv rlv G
+  : rlive_min k ZL Λ (singleton x) s sl rlv
+    -> is_rlive_min k ZL Λ (stmtLet x e s) (ann1 an sl) (Rlv \ G)
+    -> rlive_min k ZL Λ G (stmtLet x e s) (ann1 an sl) (ann1 Rlv rlv)
+| RMinIf ZL Λ e s1 s2 an sl1 sl2 Rlv rlv1 rlv2 G
+  : rlive_min k ZL Λ ∅ s1 sl1 rlv1
+    -> rlive_min k ZL Λ ∅ s2 sl2 rlv2
+    -> is_rlive_min k ZL Λ (stmtIf e s1 s2) (ann2 an sl1 sl2) (Rlv \ G)
+    -> rlive_min k ZL Λ G (stmtIf e s1 s2) (ann2 an sl1 sl2) (ann2 Rlv rlv1 rlv2)
+| RMinReturn ZL Λ e an Rlv G
+  : is_rlive_min k ZL Λ (stmtReturn e) (ann0 an) (Rlv \ G)
+    -> rlive_min k ZL Λ G (stmtReturn e) (ann0 an) (ann0 Rlv)
+| RMinApp ZL Λ f Y an Rlv G
+  : is_rlive_min k ZL Λ (stmtApp f Y) (ann0 an) (Rlv \ G)
+    -> rlive_min k ZL Λ G (stmtApp f Y) (ann0 an) (ann0 Rlv)
+| RSpillFun ZL Λ G F t spl rms sl_F sl_t Rlv rlv_F rlv_t
+  : (forall n Zs sl_s rlv_s rm,
+        get F n Zs
+        -> get sl_F n sl_s
+        -> get rlv_F n rlv_s
+        -> get rms n rm
+        -> rlive_min k (fst ⊝ F ++ ZL) (rms ++ Λ) (fst rm) (snd Zs) sl_s rlv_s)
+    -> rlive_min k (fst ⊝ F ++ ZL) (rms ++ Λ) ∅ t sl_t rlv_t
+    -> is_rlive_min k ZL Λ (stmtFun F t) (annF (spl, rms) sl_F sl_t) (Rlv \ G)
+    -> rlive_min k ZL Λ G (stmtFun F t) (annF (spl, rms) sl_F sl_t) (annF Rlv rlv_F rlv_t)
+.
+
+Lemma rlive_min_G_anti k ZL Λ G G' s sl rlv
+  : rlive_min k ZL Λ G s sl rlv
+    -> G ⊆ G'
+    -> rlive_min k ZL Λ G' s sl rlv.
+Proof.
+  intros RLM Incl.
+  general induction RLM; econstructor; intros; eauto;
+    hnf; intros; rewrite <- Incl; eauto.
+Qed.
+
+
+
+
+Lemma rlive_min_getAnn k ZL Λ s sl rlv R M :
+  rlive_min k ZL Λ ∅ s sl rlv
+  -> spill_sound k ZL Λ (R,M) s sl
+  -> getAnn rlv ⊆ R
+.
+Proof.
+  intros rliveMin spillSnd. general induction rliveMin; cbn; unfold is_rlive_min in H;
+                              rewrite <-minus_empty; try eapply H; eauto.
+Qed.
+
+Lemma rlive_min_getAnn_G k ZL Λ G s sl rlv :
+  rlive_min k ZL Λ G s sl rlv
+  -> (forall R M, spill_sound k ZL Λ (R,M) s sl -> getAnn rlv ⊆ R)
+  -> rlive_min k ZL Λ ∅ s sl rlv
+.
+Proof.
+  intros rliveMin isMin.
+  general induction rliveMin; econstructor; cbn in *; eauto;
+    unfold is_rlive_min; intros; rewrite minus_empty; eapply isMin; eauto.
+Qed.
+
+Lemma rlive_min_incl_R k ZL Λ s sl rlv R M G :
+  G ⊆ R
+  -> spill_sound k ZL Λ (R, M) s sl
+  -> rlive_min k ZL Λ G s sl rlv
+  -> getAnn rlv ⊆ R
+.
+Proof.
+  intros Geq spillSnd rlive.
+  general induction rlive; cbn;
+    unfold is_rlive_min in *; rewrite <-union_subset_equal with (s':=R); eauto;
+      apply incl_minus_incl_union; [| | | |eapply H1;eauto]; eapply H; eauto.
+Qed.
+
+Lemma rlive_min_monotone k ZL Λ s sl G G' rlv :
+  G ⊆ G'
+  -> rlive_min k ZL Λ G  s sl rlv
+  -> rlive_min k ZL Λ G' s sl rlv
+.
+Proof.
+  intros Geq rliveMin.
+  general induction rliveMin; econstructor; eauto; unfold is_rlive_min in *; intros; rewrite <-Geq;
+    eauto.
+Qed.
