theories/Spilling/RepairSpillInv.v
@@ -1,4 +1,4 @@
-Require Import RepairSpill RegLive SpillMaxKill.
+Require Import RepairSpill RLiveMin RLiveSound SpillMaxKill.
 Require Import SpillSound Annotation Liveness.Liveness RenamedApart.
 Require Import List Map IL Take TakeSet OneOrEmpty AllInRel PickLK.
 
